---
order: 3
title: Gaussian
date: 2025-07-03
categories: [BAYES, 0.probability]
tags: [Distribution, Continuous Variable, Gaussian Dist., Normal Dist.]
math: true
description: >-
    Based on the following lectures <br>
    (1) “Statistics (2018-1)” by Prof. Sang Ah Lee, Dept. of Economics, College of Economics & Commerce, Kookmin Univ. <br>
    (2) "Statistical Models and Application (2024-1)" by Prof. Yeo Jin Chung, Dept. of Data Science, The Grad. School, Kookmin Univ. <br>
    (3) “Bayesian Modeling (2024-1)” by Prof. Yeo Jin Chung, Dept. of AI, Big Data & Management, College of Business Administration, Kookmin Univ.
image:
    path: /_post_refer_img/BayesianModeling/0.Probability/Thumbnail.jpg
---

## definition
-----

![01](/_post_refer_img/BayesianModeling/0.Probability/03-01.png){: width="100%"}

- **가우시안 분포(Gaussian Distribution)**: 독립적인 무작위 충격들이 누적되어 나타나는 연속 실수값을 나타내는 분포

    $$
    X\sim\mathcal{N}(\mu,\sigma^{2})
    $$

    - $\mu$: 평균 위치로서 위치 파라미터
    - $\sigma^{2}$: 분산으로서 스케일 파라미터

- probability density function:

    $$
    p(x\mid\mu,\sigma^{2})
    =\frac{1}{\sqrt{2\pi\sigma^{2}}}\exp{\left[-\frac{(x-\mu)^{2}}{2\sigma^{2}}\right]}
    $$

- moment generating function:

    $$\begin{aligned}
    M_{X}(t)
    &=\mathbb{E}_{p(x)}\left[\exp{tX}\right]\\
    &=\int_{-\infty}^{\infty}{\exp{tx}\cdot\frac{1}{\sqrt{2\pi\sigma^{2}}}\exp{\left[-\frac{(x-\mu)^{2}}{2\sigma^{2}}\right]}\mathrm{d}x}\\
    &=\frac{1}{\sqrt{2\pi\sigma^{2}}}\int_{-\infty}^{\infty}{\exp{\left[tx-\frac{(x-\mu)^{2}}{2\sigma^{2}}\right]}\mathrm{d}x}\\
    \\
    tx-\frac{(x-\mu)^{2}}{2\sigma^{2}}
    &=-\frac{1}{2\sigma^{2}}x^{2}+\left(\frac{\mu}{\sigma^{2}}+t\right)x-\frac{\mu^{2}}{2\sigma^{2}}\\
    &=-\frac{\left[x-(\mu+\sigma^{2}+t)\right]^{2}}{2\sigma^{2}}+\mu t+\frac{\sigma^{2}t^{2}}{2}\\
    &=-\frac{\left(x-\mu^{\prime}\right)^{2}}{2\sigma^{2}}+\mu t+\frac{\sigma^{2}t^{2}}{2}\\
    \\
    \therefore M_{X}(t)
    &=\frac{1}{\sqrt{2\pi\sigma^{2}}}\int_{-\infty}^{\infty}{\exp{\left[\mu t+\frac{\sigma^{2}t^{2}}{2}\right]}\cdot\exp{\left[-\frac{(x-\mu^{\prime})^{2}}{2\sigma^{2}}\right]}\mathrm{d}x}\\
    &=\exp{\left[\mu t+\frac{\sigma^{2}t^{2}}{2}\right]}\cdot\underbrace{\frac{1}{\sqrt{2\pi\sigma^{2}}}\int_{-\infty}^{\infty}{\exp{\left[-\frac{(x-\mu^{\prime})^{2}}{2\sigma^{2}}\right]}\mathrm{d}x}}_{=1}\\
    &=\exp{\left[\mu t+\frac{\sigma^{2}t^{2}}{2}\right]}
    \end{aligned}$$

    - $\mathbb{E}\left[X\right]=(\mathrm{d}/\mathrm{d}t)M_{X}(t)\vert_{t=0}=\mu$
    - $\mathbb{E}\left[X^{2}\right]=(\mathrm{d}^{2}/\mathrm{d}t^{2})M_{X}(t)\vert_{t=0}=\mu^{2}+\sigma^{2}$
    - $\mathrm{Var}\left[X\right]=\mathbb{E}\left[X^{2}\right]-\mathbb{E}\left[X\right]^{2}=\sigma^{2}$

- canonical form ($\tau=1/\sigma^{2}$):

    $$\begin{aligned}
    p(x)
    &=\frac{1}{\sqrt{2\pi\sigma^{2}}}\exp{\left[-\frac{(x-\mu)^{2}}{2\sigma^{2}}\right]}\\
    &=\sqrt{\frac{\tau}{2\pi}}\exp{\left[-\frac{\tau}{2}(x-\mu)^{2}\right]}\\
    &=\frac{1}{\sqrt{2\pi}}\exp{\left[\begin{pmatrix}-(1/2)\tau\\\mu\tau\end{pmatrix}^{T}\begin{pmatrix}x^{2}\\x\end{pmatrix}-\frac{1}{2}(\mu^{2}\tau-\log{\tau})\right]}
    \end{aligned}$$

    - $T(x)=x^{2},x$
    - $\eta(\theta)=-(1/2)\tau,\mu\tau$
    - $A(\eta)=(1/2)(\mu^{2}\tau-\log{\tau})$
    - $h(x)=1/\sqrt{2\pi}$

## conjugate prior
-----

- gaussian model:

    $$
    X\mid\tau\sim\mathcal{N}(0,\tau^{-1})
    $$

- canonical form:

    $$\begin{aligned}
    p(x\mid\tau)
    &=\sqrt{\frac{\tau}{2\pi}}\exp{\left[-\frac{\tau}{2}x^{2}\right]}\\
    &=\frac{1}{\sqrt{2\pi}}\exp{\left[-\frac{1}{2}\tau x^{2}-\left(-\frac{1}{2}\log{\tau}\right)\right]}
    \end{aligned}$$

    - $T(x)=x^{2}$
    - $\eta(\theta)=-(1/2)\tau$
    - $A(\eta)=-(1/2)\log{\tau}$
    - $h(x)=1/\sqrt{2\pi}$

- prior of $\eta$:

    $$\begin{aligned}
    p(\eta)
    &\propto \exp\left[\alpha\cdot\eta(\theta)-\beta\cdot A(\eta)\right]\\
    &=\exp{\left[\alpha\cdot\eta-\beta\cdot\left(-\frac{1}{2}\log{[-2\eta]}\right)\right]}\\
    &=(-2\eta)^{\beta/2}\cdot\exp{\alpha\eta}
    \end{aligned}$$

- change of variables $\eta\to\tau$:

    $$\begin{aligned}
    p_{\tau}(\tau)\mathrm{d}\tau
    &=p_{\eta}(\eta)\mathrm{d}\eta\\
    \therefore p_{\tau}(\tau)
    &=p_{\eta}\left(-\frac{1}{2}\tau\right)\left\vert\frac{\mathrm{d}\eta}{\mathrm{d}\tau}\right\vert\\
    &=(\tau)^{\beta/2}\cdot\exp{\left[-\frac{\alpha}{2}\tau\right]}\cdot\frac{1}{2}\\
    &=\frac{1}{2}\tau^{(\beta/2 + 1)-1}\exp{\left[-\frac{\alpha}{2}\tau\right]}\\
    &\approx\mathrm{Gamma}\left(\frac{\beta}{2}+1,\frac{\alpha}{2}\right)
    \end{aligned}$$

- Therefore, the precision of the Gaussian distribution $1/\sigma^{2}$, the reciprocal of the variance, follows a gamma distribution. Here, each parameter of the gamma distribution represents (1) the number of virtual samples and (2) the precision scale.

    $$
    1/\sigma^{2}\sim\mathrm{Gamma}(\alpha,\beta)
    $$

## sample variance distribution
-----

- gaussian model:

    $$\begin{aligned}
    X\sim\mathcal{N}\left(\mu,\sigma^{2}\right),\quad\text{$\mu$ is known}
    \end{aligned}$$

- jeffreys prior of $\sigma^{2}$:

    $$\begin{aligned}
    p\left(\sigma^{2}\right)\propto \frac{1}{\sigma^{2}}
    \end{aligned}$$

- likelihood of $\sigma^{2}$:

    $$\begin{aligned}
    p\left(x_{1},\cdots,x_{k}\mid\sigma^{2}\right)
    &=\prod_{i=1}^{k}{p(x_{i}\mid\sigma^{2})}\quad(\because x_{i}\perp x_{j})\\
    &=\prod_{i=1}^{k}{\frac{1}{\sqrt{2\pi\sigma^{2}}}\exp{\left[-\frac{(x_{i}-\mu)^{2}}{2\sigma^{2}}\right]}}\\
    &=\prod_{i=1}^{k}{\frac{1}{\sqrt{2\pi\sigma^{2}}}}\cdot\prod_{i=1}^{k}{\exp{\left[-\frac{(x_{i}-\mu)^{2}}{2\sigma^{2}}\right]}}\\
    \\
    \prod_{i=1}^{k}{\frac{1}{\sqrt{2\pi\sigma^{2}}}}
    &=\left(2\pi\sigma^{2}\right)^{-k/2}\\
    &=(2\pi)^{-k/2}\cdot(\sigma^{2})^{-k/2}\\
    \prod_{i=1}^{k}{\exp{\left[-\frac{(x_{i}-\mu)^{2}}{2\sigma^{2}}\right]}}
    &=\exp{\left[\sum_{i=1}^{k}{-\frac{(x_{i}-\mu)^{2}}{2\sigma^{2}}}\right]}\\
    &=\exp{\left[-\frac{1}{2\sigma^{2}}\sum_{i=1}^{k}{(x_{i}-\mu)^{2}}\right]}\\
    &=\exp{\left[-\frac{1}{2}\cdot\frac{\nu S^{2}}{\sigma^{2}}\right]}\\
    \\
    \therefore p\left(x_{1},\cdots,x_{k}\mid\sigma^{2}\right)
    &=(2\pi)^{-k/2}\cdot(\sigma^{2})^{-k/2}\cdot\exp{\left[-\frac{\nu}{2\sigma^{2}}\cdot S^{2}\right]}\\
    &\propto\left(\sigma^{2}\right)^{-k/2}\cdot\exp{\left[-\frac{1}{2}\cdot\frac{\nu S^{2}}{\sigma^{2}}\right]}
    \end{aligned}$$

- posterior of $\sigma^{2}$:

    $$\begin{aligned}
    p\left(\sigma^{2}\mid x_{1},\cdots,x_{k}\right)
    &\propto p\left(x_{1},\cdots,x_{k}\mid\sigma^{2}\right)p\left(\sigma^{2}\right)\\
    &\propto\left(\sigma^{2}\right)^{-k/2}\cdot\exp{\left[-\frac{1}{2}\cdot\frac{\nu S^{2}}{\sigma^{2}}\right]}\cdot\frac{1}{\sigma^{2}}
    \end{aligned}$$

- change of variables:

    $$\begin{gathered}
    z:=\frac{\nu S^{2}}{\sigma^{2}}
    \end{gathered}$$

- posterior of $z$:

    $$\begin{aligned}
    \quad p_{z}(z)\mathrm{d}z
    &=p_{\sigma^{2}}\left(\sigma^{2}\right)\mathrm{d}\sigma^{2}\\
    \therefore p_{z}(z\mid x_{1},\cdots,x_{k})
    &\propto p_{\sigma^{2}}\left(\frac{\nu S^{2}}{z}\right)\cdot\frac{\nu S^{2}}{z^{2}}\\
    &\propto(\nu S^{2}/z)^{-k/2}\cdot\exp{\left[-\frac{\nu S^{2}}{2\nu S^{2}/z}\right]}\cdot\frac{1}{\nu S^{2}/z}\cdot\frac{\nu S^{2}}{z^{2}}\\
    &=\left(\nu S^{2}\right)^{-k/2}\cdot z^{k/2-1}\cdot\exp{\left[-\frac{1}{2}z\right]}\\
    &\approx z^{k/2-1}\cdot\exp{\left[-\frac{1}{2}z\right]}\\
    &\approx \chi^{2}(k)
    \end{aligned}$$

- therefore, **sample variance** of gaussian distribution, $S^{2}$, follows a chi-square distribution.

    $$\begin{aligned}
    z=\frac{\nu S^{2}}{\sigma^{2}}=\sum_{i=1}^{k}{\left(\frac{x_{i}-\mu}{\sigma}\right)^{2}}
    \sim\chi^{2}(k)
    \end{aligned}$$

## student's t
-----

![05](/_post_refer_img/BayesianModeling/0.Probability/03-05.png){: width="100%"}

- gaussian random variable:

    $$
    X_{i}\sim\mathcal{N}(\mu,\sigma^{2})
    $$

- standardization:

    $$
    Z=\frac{\overline{X}-\mu}{\sigma/\sqrt{n}}\sim\mathcal{N}(0,1)
    $$

- If the population variance $\sigma^{2}$ is unknown, the sample variance $S^{2}$ can be used:

    $$
    S^{2}=\frac{1}{\nu}\sum_{i=1}^{n}{\left(X_{i}-\overline{X}\right)^{2}}
    $$

- chi-squared dist.:

    $$\begin{aligned}
    U\sim\chi^{2}(\nu)
    \end{aligned}$$

- chi-squared variable can be represented by $S^{2}$:

    $$\begin{aligned}
    U
    &=\sum_{i=1}^{n}{\left(\frac{X_{i}-\overline{X}}{\sigma}\right)^{2}}\\
    &=\frac{1}{\sigma^{2}}\cdot\nu S^{2}
    \end{aligned}$$

- as a result, when the population variance is unknown, the test statistic can be replaced by the ratio of the chi-square random variable to the standard normal random variable:

    $$\begin{aligned}
    \frac{\overline{X}-\mu}{S/\sqrt{n}}
    &=\underbrace{\frac{\overline{X}-\mu}{\sigma/\sqrt{n}}}_{=:Z}\cdot\frac{\sigma}{S}\\
    &=Z\cdot\frac{1}{\sqrt{S^{2}/\sigma^{2}}}\\
    &=\frac{Z}{\sqrt{U/\nu}}\quad\left(\because\frac{S^{2}}{\sigma^{2}}=\frac{U}{\nu}\right)
    \end{aligned}$$

- the ratio of the chi-square random variable to the standard normal random variable is defined as the Student's t random variable:

    $$
    T=\frac{Z}{\sqrt{U/\nu}}\sim t(\nu),\quad Z \perp U
    $$